CredibleCompilation/DCEOpt.lean
@@ -145,7 +145,7 @@ def buildInstrCerts (origMap : Array Nat) (trans : Prog) : Array EInstrCert :=
 
 /-- Run dead code elimination on `prog` and produce a certified transformation.
     The result is an `ECertificate` that `checkCertificateExec` will accept. -/
-def optimize (prog : Prog) (observable : List Var) : ECertificate :=
+def optimize (prog : Prog) : ECertificate :=
   let consts := ConstPropOpt.analyze prog
   let reached := reachable prog consts
   let origMap := _root_.buildOrigMap reached
@@ -157,10 +157,8 @@ def optimize (prog : Prog) (observable : List Var) : ECertificate :=
   let haltCerts := _root_.buildHaltCerts instrCerts trans
   { orig := prog
     trans := trans
-    tyCtx := fun _ => VarTy.int
     inv_orig := inv_orig
     inv_trans := inv_trans
-    observable := observable
     instrCerts := instrCerts
     haltCerts := haltCerts
     measure := Array.replicate trans.size 0 }
