CredibleCompilation/PeepholeOptExamples.lean
@@ -36,18 +36,19 @@ namespace PeepholeOptExamples
     6: goto 2
 -/
 
-def licmProg : Prog := .ofCode #[
-  .const "one" (.int 1),
-  .binop "t" .mul "a" "b",
-  .ifgoto (.cmpLit .ne "n" 0) 4,
-  .halt,
-  .binop "s" .add "s" "t",
-  .goto 6,
-  .binop "n" .sub "n" "one",
-  .goto 2
-]
+def licmProg : Prog :=
+  { code := #[
+      .const "one" (.int 1),
+      .binop "t" .mul "a" "b",
+      .ifgoto (.cmpLit .ne "n" 0) 4,
+      .halt,
+      .binop "s" .add "s" "t",
+      .goto 6,
+      .binop "n" .sub "n" "one",
+      .goto 2
+    ], tyCtx := fun _ => .int, observable := ["s"] }
 
-def licmCert := optimize licmProg ("s" :: [])
+def licmCert := optimize licmProg
 
 #eval! licmCert.trans
 #eval! checkCertificateExec licmCert
@@ -69,14 +70,15 @@ def licmCert := optimize licmProg ("s" :: [])
     2: halt
 -/
 
-def selfCopyProg : Prog := .ofCode #[
-  .const "x" (.int 5),
-  .copy "x" "x",
-  .const "y" (.int 3),
-  .halt
-]
+def selfCopyProg : Prog :=
+  { code := #[
+      .const "x" (.int 5),
+      .copy "x" "x",
+      .const "y" (.int 3),
+      .halt
+    ], tyCtx := fun _ => .int, observable := ["x", "y"] }
 
-def selfCopyCert := optimize selfCopyProg ("x" :: "y" :: [])
+def selfCopyCert := optimize selfCopyProg
 
 #eval! selfCopyCert.trans
 #eval! checkCertificateExec selfCopyCert
@@ -100,16 +102,17 @@ def selfCopyCert := optimize selfCopyProg ("x" :: "y" :: [])
     2: halt
 -/
 
-def chainNopProg : Prog := .ofCode #[
-  .const "x" (.int 1),
-  .goto 2,
-  .goto 3,
-  .goto 4,
-  .const "y" (.int 2),
-  .halt
-]
+def chainNopProg : Prog :=
+  { code := #[
+      .const "x" (.int 1),
+      .goto 2,
+      .goto 3,
+      .goto 4,
+      .const "y" (.int 2),
+      .halt
+    ], tyCtx := fun _ => .int, observable := ["x", "y"] }
 
-def chainNopCert := optimize chainNopProg ("x" :: "y" :: [])
+def chainNopCert := optimize chainNopProg
 
 #eval! chainNopCert.trans
 #eval! checkCertificateExec chainNopCert
@@ -128,14 +131,15 @@ def chainNopCert := optimize chainNopProg ("x" :: "y" :: [])
   Expected: unchanged
 -/
 
-def noChangeProg : Prog := .ofCode #[
-  .const "x" (.int 5),
-  .const "y" (.int 3),
-  .binop "z" .add "x" "y",
-  .halt
-]
+def noChangeProg : Prog :=
+  { code := #[
+      .const "x" (.int 5),
+      .const "y" (.int 3),
+      .binop "z" .add "x" "y",
+      .halt
+    ], tyCtx := fun _ => .int, observable := ["z"] }
 
-def noChangeCert := optimize noChangeProg ("z" :: [])
+def noChangeCert := optimize noChangeProg
 
 #eval! noChangeCert.trans
 #eval! checkCertificateExec noChangeCert
@@ -159,15 +163,16 @@ def noChangeCert := optimize noChangeProg ("z" :: [])
     3: halt
 -/
 
-def gotoToNopProg : Prog := .ofCode #[
-  .const "x" (.int 1),
-  .goto 3,
-  .goto 3,
-  .const "y" (.int 2),
-  .halt
-]
+def gotoToNopProg : Prog :=
+  { code := #[
+      .const "x" (.int 1),
+      .goto 3,
+      .goto 3,
+      .const "y" (.int 2),
+      .halt
+    ], tyCtx := fun _ => .int, observable := ["x", "y"] }
 
-def gotoToNopCert := optimize gotoToNopProg ("x" :: "y" :: [])
+def gotoToNopCert := optimize gotoToNopProg
 
 #eval! gotoToNopCert.trans
 #eval! checkCertificateExec gotoToNopCert
@@ -189,14 +194,15 @@ def gotoToNopCert := optimize gotoToNopProg ("x" :: "y" :: [])
     2: halt
 -/
 
-def ifgotoNopProg : Prog := .ofCode #[
-  .ifgoto (.cmpLit .lt "x" 10) 3,
-  .goto 2,
-  .const "a" (.int 1),
-  .halt
-]
+def ifgotoNopProg : Prog :=
+  { code := #[
+      .ifgoto (.cmpLit .lt "x" 10) 3,
+      .goto 2,
+      .const "a" (.int 1),
+      .halt
+    ], tyCtx := fun _ => .int, observable := ["a"] }
 
-def ifgotoNopCert := optimize ifgotoNopProg ("a" :: [])
+def ifgotoNopCert := optimize ifgotoNopProg
 
 #eval! ifgotoNopCert.trans
 #eval! checkCertificateExec ifgotoNopCert
@@ -210,22 +216,23 @@ def ifgotoNopCert := optimize ifgotoNopProg ("a" :: [])
     This demonstrates the optimizer pipeline.
 -/
 
-def e2eProg : Prog := .ofCode #[
-  .const "one" (.int 1),
-  .binop "t" .mul "a" "b",
-  .ifgoto (.cmpLit .ne "n" 0) 4,
-  .halt,
-  .binop "s" .add "s" "t",
-  .binop "t" .mul "a" "b",
-  .binop "n" .sub "n" "one",
-  .goto 2
-]
+def e2eProg : Prog :=
+  { code := #[
+      .const "one" (.int 1),
+      .binop "t" .mul "a" "b",
+      .ifgoto (.cmpLit .ne "n" 0) 4,
+      .halt,
+      .binop "s" .add "s" "t",
+      .binop "t" .mul "a" "b",
+      .binop "n" .sub "n" "one",
+      .goto 2
+    ], tyCtx := fun _ => .int, observable := ["s"] }
 
 -- Step 1: LICM removes redundant t := a*b (becomes goto 6)
-def e2eLicm := LICMOpt.optimize e2eProg ("s" :: [])
+def e2eLicm := LICMOpt.optimize e2eProg
 
 -- Step 2: Peephole removes the goto 6 left by LICM
-def e2ePeep := optimize e2eLicm.trans ("s" :: [])
+def e2ePeep := optimize e2eLicm.trans
 
 #eval! e2eLicm.trans    -- after LICM: has goto 6
 #eval! e2ePeep.trans    -- after peephole: goto 6 removed
